\documentclass{article}
\usepackage{amsmath}
\usepackage{amssymb}
\usepackage{amsthm}
\usepackage[T1]{fontenc}


\newtheorem*{conjecture}{Przypuszczenie}
\newtheorem*{theorem}{Twierdzenie}
\newtheorem{lemma}{Lemat}
\renewcommand*{\proofname}{Dowód}


\makeatletter
\newcommand*{\rom}[1]{\expandafter\@slowromancap\romannumeral #1@}
\makeatother


\DeclareMathOperator{\interior}{int}

\begin{document}

\section{Część A}

\subsection{Obliczyć granice}

\subsubsection*{4}

\begin{equation*}
    \lim_{x \to 1} \frac{1 - \sqrt[3]{x}}{1 - \sqrt[5]{x}} = \lim_{x \to 1} \frac{1 - \sqrt[3]{x}}{1 - \sqrt[5]{x}}\Bigg(\frac{(1 + \sqrt[3]{x} + \sqrt[3]{x}^2)}{(1 + \sqrt[3]{x} + \sqrt[3]{x}^2)}\Bigg) =
\end{equation*}
\begin{equation*}
    = \lim_{x \to 1} \frac{1 - \sqrt[3]{x}}{1 - \sqrt[5]{x}} \Bigg(\frac{(1 + \sqrt[3]{x} + \sqrt[3]{x}^2)}{(1 + \sqrt[3]{x} + \sqrt[3]{x}^2)}\Bigg) \Bigg(\frac{1 + \sqrt[5]{x} + \sqrt[5]{x}^2 + \sqrt[5]{x}^3 + \sqrt[5]{x}^4}{1 + \sqrt[5]{x} + \sqrt[5]{x}^2 + \sqrt[5]{x}^3 + \sqrt[5]{x}^4}\Bigg)
\end{equation*}
\begin{equation*}
    = \lim_{x \to 1} \frac{(1 - x)(1 + \sqrt[5]{x} + \sqrt[5]{x}^2 + \sqrt[5]{x}^3 + \sqrt[5]{x}^4)}{(1 - x)(1 + \sqrt[3]{x} + \sqrt[3]{x}^2)}
\end{equation*}
\begin{equation*}
    = \lim_{x \to 1} \frac{(1 + \sqrt[5]{x} + \sqrt[5]{x}^2 + \sqrt[5]{x}^3 + \sqrt[5]{x}^4)}{(1 + \sqrt[3]{x} + \sqrt[3]{x}^2)}
\end{equation*}
\begin{equation*}
    = \frac{1 + \sqrt[5]{1} + \sqrt[5]{1^2} + \sqrt[5]{1^3} + \sqrt[5]{1^4}}{1 + \sqrt[3]{1} + \sqrt[3]{1^2}} = \frac{5}{3}
\end{equation*}

\subsubsection*{5}

\begin{equation*}
    \lim_{x \to 0} \frac{\sqrt{x^2 + 1} - \sqrt{x + 1}}{1 - \sqrt{x + 1}} = \lim_{x \to 0} \Bigg(\frac{\sqrt{x^2 + 1} - \sqrt{x + 1}}{1 - \sqrt{x + 1}}\Bigg) \Bigg(\frac{1 + \sqrt{x + 1}}{1 + \sqrt{x + 1}}\Bigg)
\end{equation*}
\begin{equation*}
    = \lim_{x \to 0} \frac{\Big(\sqrt{x^2 + 1} - \sqrt{x + 1}\Big)(1 + \sqrt{x + 1})}{1 - x - 1}
\end{equation*}
\begin{equation*}
    = \lim_{x \to 0} \frac{\Big(\sqrt{x^2 + 1} - \sqrt{x + 1}\Big)(1 + \sqrt{x + 1})}{-x}
\end{equation*}
\begin{equation*}
    = \lim_{x \to 0} \frac{\Big(\sqrt{x^2 + 1} - \sqrt{x + 1}\Big)(1 + \sqrt{x + 1})}{-x} \frac{(\sqrt{x^2 + 1} + \sqrt{x + 1})}{(\sqrt{x^2 + 1} + \sqrt{x + 1})}
\end{equation*}
\begin{equation*}
    = \lim_{x \to 0} \frac{(x^2 + 1 -x - 1)(1 + \sqrt{x + 1})}{-x(\sqrt{x^2 + 1} + \sqrt{x + 1})}
\end{equation*}
\begin{equation*}
    = \lim_{x \to 0} \frac{-x(1 - x)(1 + \sqrt{x + 1})}{-x(\sqrt{x^2 + 1} + \sqrt{x + 1})}
\end{equation*}
\begin{equation*}
    = \lim_{x \to 0} \frac{(1 - x)(1 + \sqrt{x + 1})}{(\sqrt{x^2 + 1} + \sqrt{x + 1})}
\end{equation*}
\begin{equation*}
    = \frac{(1 - 0)(1 + \sqrt{0 + 1})}{(\sqrt{0^2 + 1} + \sqrt{0 + 1})} = \frac{(1 + 1)}{(1 + 1)} = \frac{2}{2} = 1
\end{equation*}


\subsubsection*{6}

\begin{equation*}
    \lim_{x \to -\infty} (\sqrt{x^2 -8x + 3} - \sqrt{x^2 +11x}) 
\end{equation*}
\begin{equation*}
    = \lim_{x \to -\infty} (\sqrt{x^2 -8x + 3} - \sqrt{x^2 +11x}) \frac{(\sqrt{x^2 -8x + 3} + \sqrt{x^2 +11x})}{(\sqrt{x^2 -8x + 3} + \sqrt{x^2 +11x})} 
\end{equation*}
\begin{equation*}
    = \lim_{x \to -\infty} \frac{x^2 -8x + 3 -x^2 - 11x}{(\sqrt{x^2 -8x + 3} + \sqrt{x^2 +11x})}
\end{equation*}
\begin{equation*}
    = \lim_{x \to -\infty} \frac{-19x + 3}{(\sqrt{x^2 -8x + 3} + \sqrt{x^2 +11x})}
\end{equation*}


\end{document}