\documentclass{article}
\usepackage{amsmath}
\usepackage{amssymb}
\usepackage{amsthm}


\newtheorem*{conjecture}{Conjecture}
\newtheorem*{theorem}{Theorem}


\makeatletter
\newcommand*{\rom}[1]{\expandafter\@slowromancap\romannumeral #1@}
\makeatother


\begin{document}

\section*{1-1}

We will use field axioms in \(\mathbb{R}\)  to show that \((-1)(-1) = 1\). First let us observe that:

\begin{equation*}
    0 = (-1) \cdot 0  \ \ \ \mbox{\emph{A neutral element 1 for multiplication}}
\end{equation*}
\begin{equation*}
    = (-1) \cdot (1 + (-1)) \ \ \ \mbox{\emph{Additive inverse}}
\end{equation*}
\begin{equation*}
    = (-1) \cdot 1 + (-1) \cdot (-1) \ \ \ \mbox{\emph{Left distributivity of addition}}
\end{equation*}
\begin{equation*}
    = 1 \cdot (-1) + (-1) \cdot (-1) \ \ \ \mbox{\emph{Commutativity of multiplication}}
\end{equation*}
\begin{equation*}
    = (-1) + (-1) \cdot (-1) \ \ \ \mbox{\emph{A neutral element 1 for multiplication}}
\end{equation*}

We end up with the following equation:
\begin{equation*}
    (-1) + (-1) \cdot (-1) = 0
\end{equation*}
Adding \(1\) on both sides and using \emph{Additive inverse} and \emph{Associativity of addition}:
\begin{equation*}
    (1 + (-1)) + (-1)(-1) = 0 + (-1)(-1) = (-1)(-1) = 1
\end{equation*}

\section*{1-2}

Let \(x, y, z \in \mathbb{R}\). We need to prove that:
\begin{equation*}
    (x + y)z = xz = yz
\end{equation*}
knowing from our field axioms that operation \((\cdot)\) is \emph{left} distributive. Let us make an observation
that by definition of field, \( (x + y) \in \mathbb{R}\). This means that \((x+y)z = z(x+y)\) because of \emph{Commutativity of multiplication}.
And then using \emph{Left distributivity of addition} we arrive to:
\begin{equation*}
    (x+y)z = z(x+y) = zx + zy
\end{equation*}

\section*{1-3}

Let \(x \in \mathbb{R}\) and \(x', \  \overline{x}\) be multiplicative inverses of \(x\). 
We will show that multiplicative inverses are unique:

\begin{equation*}
    x' = 1 \cdot x' \ \ \ \mbox{\emph{A neutral element 1 for multiplication}}
\end{equation*}
\begin{equation*}
    = (x \overline{x}) \cdot x' \ \ \ \mbox{\emph{Multiplicative inverse}}
\end{equation*}
\begin{equation*}
    = (\overline{x} x) \cdot x' \ \ \ \mbox{\emph{Commutativity of multiplication}}
\end{equation*}
\begin{equation*}
    = \overline{x} \cdot (xx') \ \ \ \mbox{\emph{Associativity of multiplication}}
\end{equation*}
\begin{equation*}
    = \overline{x} \cdot 1 \ \ \ \mbox{\emph{Multiplicative inverse}}
\end{equation*}
\begin{equation*}
    = \overline{x} \ \ \ \mbox{\emph{A neutral element 1 for multiplication}}
\end{equation*}

We have shown that \(\overline{x} = x'\) which means that if multiplicative inverse exists, it is unique.

\section*{1-4}

If \(0\) had a multiplicative inverse then we would have \(0 \cdot 0^{-1} = 1\). But that 
would mean that we could multiply an element of reals field \(0^{-1}\) by \(0\). According to
the field axioms we should have then had \(0^{-1} \cdot 0 = 0\) but this would contradict our
assumption that \(0 \cdot 0^{-1} = 1\).

\section*{1-5}

We know that \((xy)\) is invertible because we start with the assumption that \(x \neq 0\) and \(y \neq 0\).
Which means that \(x \cdot y \neq 0\). Hence, \(xy\) is some real number, and from axioms we know that
every real number other than zero has an inverse.  

Let us first use \emph{Existence of multiplicative inverses} to settle the ground for our proof:
\begin{equation*}
	(xy)^{-1}(xy) = 1
\end{equation*}
Now we will use the chain of properties of real numbers:
\begin{equation*}
	(xy)^{-1}(xy) = 1 \cdot 1 \ \ \ \emph{Existence of the multiplicative identity}
\end{equation*}
\begin{equation*}
	(xy)^{-1}(xy) = (x^{-1}x) \cdot (yy^{-1}) \ \ \ \emph{Existence of multiplicative inverses}
\end{equation*}
\begin{equation*}
	(xy)^{-1}(xy) = (x^{-1}y^{-1}) \cdot (xy) \ \ \ \emph{Associative and commutative laws for multiplication (lots of)} 
\end{equation*}
\begin{equation*}
	(xy)^{-1} = (x^{-1}y^{-1}) \ \ \ \emph{Existence of multiplicative inverses and associative law for multiplication} 
\end{equation*}
and our proof is done (see also Spivak Chapter 1 3.(iii)).


\section*{1-6}

\subsection*{(a)}
We will prove the following formula:
\begin{equation*}
    (a + b)^2 = a^2 + 2ab + b^2
\end{equation*}
Let us justify each step using field axioms of \(\mathbb{R}\):
\begin{equation*}
    (a + b)^2 = (a + b)(a + b) \ \ \ \mbox{\emph{Definition of exponentiation}}
\end{equation*}
\begin{equation*}
    = \Big(a \cdot (a + b)\Big) + \Big(b \cdot (a + b)\Big) \ \ \ \mbox{\emph{Distributivity over addition}}
\end{equation*}
\begin{equation*}
    = \Big( (a \cdot a) + (a \cdot b)\Big) + \Big( (b \cdot a) + (b \cdot b)\Big) \ \ \ \mbox{\emph{Distributivity over addition}} 
\end{equation*}
\begin{equation*}
    = \Big( a^2 + (a \cdot b)\Big) + \Big( (b \cdot a) + b^{2}\Big) \ \ \ \mbox{\emph{Definition of exponentiation}} 
\end{equation*}
\begin{equation*}
    = \Big( a^2 + (a \cdot b)\Big) + \Big( (a \cdot b) + b^{2}\Big) \ \ \ \mbox{\emph{Commutativity of multiplication}} 
\end{equation*}
\begin{equation*}
    = \Bigg(\Big(a^2 + (a \cdot b)\Big) + (a \cdot b)\Bigg)  + \Big(b^{2}\Big) \ \ \ \mbox{\emph{Associativity of addition}} 
\end{equation*}
\begin{equation*}
    = \Bigg(\Big(a^2 + 2a b)\Big)\Bigg)  + \Big(b^{2}\Big) \ \ \ \mbox{\emph{Associativity of addition}} 
\end{equation*}
\begin{equation*}
    = a^2 + 2ab + b^2
\end{equation*}

\subsection*{(b)}

We will prove the following formula:
\begin{equation*}
    (a - b)^2 = a^2 - 2ab + b^2
\end{equation*}
Let us justify each step using field axioms of \(\mathbb{R}\):
\begin{equation*}
    \Big(a + (-b)\Big)^2 = \Big(a + (-b)\Big) \Big(a + (-b)\Big) \ \ \ \mbox{\emph{Definition of exponentiation}}
\end{equation*}
\begin{equation*}
    = \Big(a \cdot a + a \cdot (-b)\Big) + \Big((-b) \cdot a + (-b) \cdot (-b)\Big) \ \ \ \mbox{\emph{Distributivity over addition}}
\end{equation*}
\begin{equation*}
    = \Bigg(a^2 + \Big(a \cdot (-b)\Big)\Bigg) + \Bigg(\Big( (-b) \cdot a \Big) + b^2 \Bigg) \ \ \ \mbox{\emph{Definition of exponentiation}}
\end{equation*}
\begin{equation*}
    =   \Bigg(a^2 + \Big(a \cdot (-b)\Big) + \Big( (-b) \cdot a \Big) \Bigg) + \Bigg(b^2 \Bigg) \ \ \ \mbox{\emph{Associativity of addition}}
\end{equation*}
\begin{equation*}
    = \Bigg(a^2 + 2 \Big(a \cdot (-b)\Big) \Bigg) + \Bigg(b^2 \Bigg) = a^2 -2ab + b^2
\end{equation*}
where in the last step we just present our result in a more convienient notation. With that the proof is done.


\subsection*{(c)}

We will prove the following formula:
\begin{equation*}
    (a + b)(a - b) = a^2 - b^2
\end{equation*}
\newline
\begin{equation*}
    (a + b)(a - b) = (a + b)(a +  (-b))
\end{equation*}
\begin{equation*}
    = \Big( a \cdot a + \big(a \cdot (-b)\big)\Big) + \Big( b \cdot a + \big(b \cdot (-b)\big)\Big) \ \ \ \mbox{\emph{Distributivity over addition}}
\end{equation*}
\begin{equation*}
    = \Big( a^2 + \big(a \cdot (-b)\big)\Big) + \Big( b \cdot a + (-b^2) \Big) \ \ \ \mbox{\emph{Definition of exponentiation}}
\end{equation*}
\begin{equation*}
    = \Big( a^2 + \big(a \cdot (-b)\big) + b \cdot a \Big) + (-b^2)  \ \ \ \mbox{\emph{Associativity of addition}}
\end{equation*}
\begin{equation*}
    = \Big( a^2 + 0 \Big) + (-b^2)  \ \ \ \mbox{\emph{Existence of additive inverses}}
\end{equation*}
\begin{equation*}
    = a^2  + (-b^2) = a^2 - b^2  \ \ \ \mbox{\emph{Neutral element for addition}}
\end{equation*}
As shown by field axioms it follows that \((a + b)(a - b) = a^2 - b^2 \)

\section*{1-10}
\subsection*{(a)}
\subsubsection*{\(x\) is positive}

Let \(x\) be positive. Then \(x \in \mathbb{R^{+}}\). We want to show that:

\begin{equation*}
    x > 0 \iff 0 < x \iff (x - 0) \in \mathbb{R^{+}}
\end{equation*}

Observe that by the field axioms of reals:

\begin{equation*}
    x - 0 = x + (-0) = x + ((-1) \cdot 0) = x + 0 = x 
\end{equation*}

From our initial assumption we know that \(x\) is positive, hence \(x - 0\) is also positive and
that concludes the proof in one direction. For the other direction, assume now that \(x > 0\). It means then that
\((x - 0) \in \mathbb{R^{+}}\). Again, from the observation above, this is just an equivalent way of saying that
\(x \in \mathbb{R^{+}}\), so \(x\) is positive.

\subsubsection*{\(x\) is negative}

Let \(x\) be negative. Then \(-x \in \mathbb{R^{+}}\). Using the same observation from the positive case above:
\begin{equation*}
    (0 - x) = 0 + (-x) = -x \in \mathbb{R^{+}}
\end{equation*}
And so, if \((0 - x) = -x\) and \(-x \in \mathbb{R^{+}}\) it follows that \(x < 0\). For the opposite direction, assume that
\(x < 0\). Then \((0 - x) \in \mathbb{R^{+}}\). From here, one can easily see that \((-x) \in \mathbb{R^{+}}\)

\subsection*{(b)}

Let \(x, y, z \in \mathbb{R^{+}}\) and let \(x \leq y\). For the first case, assume that \(x = y\). Then from the definition it is clear
to see that \(x \leq y\). Assume now that \(x < y\). Then \((y - x) \) is a positive real number.  We need to show that \(x + z \leq y + z\). In other words, we need to show that
\((y + z) - (x + z)\) is a positive real number. From the field axioms of reals we see that:
\begin{equation*}
    (y + z) - (x + z) = (y + z) + (-(x + z)) = (y + z) + (-x - z) = y + 0 - x = y - x
\end{equation*} 
But we know that this is a positive real number from \(x < y\). Thus \( \Big((y + z) - (x + z)\Big) \in \mathbb{R^{+}}\) and \(x + z \leq y + z\).

\end{document}
